ok

SStructTT/SStruct/Erasure/Step.lean
@@ -19,41 +19,105 @@ inductive Value : Tm Srt -> Prop where
   | null : Value .null
 
 @[scoped aesop safe [constructors]]
-inductive Step : Tm Srt -> Tm Srt -> Prop where
+inductive Step0 : Tm Srt -> Tm Srt -> Prop where
   | app_M {m m'} n :
-    Step m m' ->
-    Step (.app m n) (.app m' n)
+    Step0 m m' ->
+    Step0 (.app m n) (.app m' n)
   | app_N m {n n'} :
-    Step n n' ->
-    Step (.app m n) (.app m n')
+    Step0 n n' ->
+    Step0 (.app m n) (.app m n')
+  | tup_M {m m'} n s :
+    Step0 m m' ->
+    Step0 (.tup m n s) (.tup m' n s)
+  | tup_N m {n n'} s :
+    Step0 n n' ->
+    Step0 (.tup m n s) (.tup m n' s)
+  | prj_M {m m'} n :
+    Step0 m m' ->
+    Step0 (.prj m n) (.prj m' n)
+  | ite_M {m m'} n1 n2 :
+    Step0 m m' ->
+    Step0 (.ite m n1 n2) (.ite m' n1 n2)
+  | drop_elim m n :
+    Step0 (.drop m n) n
+
+@[scoped aesop safe [constructors]]
+inductive Step1 : Tm Srt -> Tm Srt -> Prop where
+  | app_M {m m'} n :
+    Step1 m m' ->
+    Step1 (.app m n) (.app m' n)
+  | app_N m {n n'} :
+    Step1 n n' ->
+    Step1 (.app m n) (.app m n')
   | beta m n s :
     Value n ->
-    Step (.app (.lam m s) n) m.[n/]
+    Step1 (.app (.lam m s) n) m.[n/]
   | tup_M {m m'} n s :
-    Step m m' ->
-    Step (.tup m n s) (.tup m' n s)
+    Step1 m m' ->
+    Step1 (.tup m n s) (.tup m' n s)
   | tup_N m {n n'} s :
-    Step n n' ->
-    Step (.tup m n s) (.tup m n' s)
+    Step1 n n' ->
+    Step1 (.tup m n s) (.tup m n' s)
   | prj_M {m m'} n :
-    Step m m' ->
-    Step (.prj m n) (.prj m' n)
+    Step1 m m' ->
+    Step1 (.prj m n) (.prj m' n)
   | prj_elim {m1 m2} n {s} :
     Value (.tup m1 m2 s) ->
-    Step (.prj (.tup m1 m2 s) n) n.[m2,m1/]
+    Step1 (.prj (.tup m1 m2 s) n) n.[m2,m1/]
   | ite_M {m m'} n1 n2 :
-    Step m m' ->
-    Step (.ite m n1 n2) (.ite m' n1 n2)
+    Step1 m m' ->
+    Step1 (.ite m n1 n2) (.ite m' n1 n2)
   | ite_tt n1 n2 :
-    Step (.ite .tt n1 n2) n1
+    Step1 (.ite .tt n1 n2) n1
   | ite_ff n1 n2 :
-    Step (.ite .ff n1 n2) n2
+    Step1 (.ite .ff n1 n2) n2
   | rw_elim m :
-    Step (.rw m) m
+    Step1 (.rw m) m
+
+def Step (m : Tm Srt) (n : Tm Srt) : Prop :=
+  Step0 m n ∨ Step1 m n
 
 notation:50 m:50 " ~>> " n:50 => Step m n
 notation:50 m:50 " ~>>* " n:50 => ARS.Star Step m n
 
-inductive StepDrop : Tm Srt -> Tm Srt -> Prop where
-  | drop_elim m n :
-    StepDrop (.drop m n) n
+lemma Step.app_M {m m' n : Tm Srt} :
+    m ~>> m' -> .app m n ~>> .app m' n := by
+  intro st
+  cases st with
+  | inl st => left; constructor; assumption
+  | inr st => right; constructor; assumption
+
+lemma Step.app_N {m n n' : Tm Srt} :
+    n ~>> n' -> .app m n ~>> .app m n' := by
+  intro st
+  cases st with
+  | inl st => left; constructor; assumption
+  | inr st => right; constructor; assumption
+
+lemma Step.tup_M {m m' n : Tm Srt} {s} :
+    m ~>> m' -> .tup m n s ~>> .tup m' n s := by
+  intro st
+  cases st with
+  | inl st => left; constructor; assumption
+  | inr st => right; constructor; assumption
+
+lemma Step.tup_N {m n n' : Tm Srt} {s} :
+    n ~>> n' -> .tup m n s ~>> .tup m n' s := by
+  intro st
+  cases st with
+  | inl st => left; constructor; assumption
+  | inr st => right; constructor; assumption
+
+lemma Step.prj_M {m m' n : Tm Srt} :
+    m ~>> m' -> .prj m n ~>> .prj m' n := by
+  intro st
+  cases st with
+  | inl st => left; constructor; assumption
+  | inr st => right; constructor; assumption
+
+lemma Step.ite_M {m m' n1 n2 : Tm Srt} :
+    m ~>> m' -> .ite m n1 n2 ~>> .ite m' n1 n2 := by
+  intro st
+  cases st with
+  | inl st => left; constructor; assumption
+  | inr st => right; constructor; assumption
